

SUMS OF POWERS VIA BACKWARD FINITE DIFFERENCES AND NEWTON'S FORMULA

PETRO KOLOSOV

ABSTRACT. We obtain formulas for sums of powers via Newton's interpolation formula based on backward finite differences of powers. In addition, we note that backward differences are closely related to Eulerian numbers, and Stirling numbers of the second kind. Thus, we express formulas for sums of powers in terms of Eulerian numbers, and Stirling numbers of the second kind.

CONTENTS

Abstract	1
1. Introduction and main results	1
2. Conclusions	6
References	7
Mathematica programs	8

1. INTRODUCTION AND MAIN RESULTS

In this manuscript, we obtain formulas for sums of powers via Newton's interpolation formula based on backward finite differences of powers. The idea to derive sums of powers

Date: January 3, 2026.

2010 Mathematics Subject Classification. 05A19, 05A10, 11B68, 11B73, 11B83.

Key words and phrases. Sums of powers, Newton's interpolation formula, Finite differences, Binomial coefficients, Faulhaber's formula, Bernoulli numbers, Bernoulli polynomials, Interpolation, Discrete convolution, Combinatorics, Polynomial identities, Central factorial numbers, Stirling numbers, Eulerian numbers, Worpitzky identity, Pascal's triangle, OEIS.

DOI: <https://doi.org/10.5281/zenodo.18118011>

using difference operator and Newton's series is quite generic, thus, formulas for sums of powers using forward and central differences can be found in the works [1, 2].

Define multifold sums of powers in Knuth's [3] notation

$$\Sigma^0 n^m = n^m$$

$$\Sigma^1 n^m = \Sigma^0 1^m + \Sigma^0 2^m + \cdots + \Sigma^0 n^m$$

$$\Sigma^{r+1} n^m = \Sigma^r 1^m + \Sigma^r 2^m + \cdots + \Sigma^r n^m$$

The book Interpolation by Steffensen [4, chapter 2, eq. (19)] gives Newton's formula for backward differences evaluated in zero $f(x) = \sum_{k=0}^n \binom{x+k-1}{k} \nabla^k f(0)$.

In general,

Proposition 1.1 (Newton formula via backward differences).

$$f(x) = \sum_{k=0}^n \binom{x-a+k-1}{k} \nabla^k f(a)$$

where $\nabla^k f(a) = \sum_{j=0}^k (-1)^j \binom{k}{j} f(a-j)$.

Thus, by setting $f(n) = n^m$

$$n^m = \sum_{j=0}^m \binom{n-t+j-1}{j} \nabla^j t^m,$$

where $\nabla^j t^m = \sum_{k=0}^j (-1)^k \binom{j}{k} (t-k)^m$. Therefore, ordinary sums of powers is equivalent to

$$\Sigma^1 n^m = \sum_{j=0}^m \nabla^j t^m \sum_{k=1}^n \binom{k-t+j-1}{j}$$

We notice that the sum $\sum_{k=1}^n \binom{k-t+j-1}{j}$ is a good candidate for hockey stick identity for binomial coefficients $\sum_{k=0}^n \binom{k}{j} = \binom{n+1}{j+1}$. Thus, by setting $a = j-t$ and $b = j-t-1+n$, we get

$$\sum_{k=1}^n \binom{-t+j-1+k}{j} = \sum_{m=j-t}^{j-t-1+n} \binom{m}{j}$$

Thus,

$$\sum_{k=1}^n \binom{-t+j-1+k}{j} = \binom{j-t+n}{j+1} - \binom{j-t}{j+1}$$

Because,

Lemma 1.2 (Generalized hockey stick identity).

$$\sum_{m=a}^b \binom{m}{j} = \binom{b+1}{j+1} - \binom{a}{j+1}$$

Applying the identity for binomial coefficients $\binom{-k}{j} = (-1)^j \binom{j+k-1}{j}$, we obtain

Proposition 1.3 (Ordinary sums of powers via backward differences). *For non-negative integers n, m and an arbitrary integer t*

$$\Sigma^1 n^m = \sum_{j=0}^m \nabla^j t^m \left[(-1)^j \binom{t}{j+1} + \binom{j-t+n}{j+1} \right]$$

For example, by setting $t = 2$ and $m = 1, 2, 3, 4$, we get formulas for sums of cubes

$$\Sigma^1 n^1 = 2 \left[-\binom{2}{1} + \binom{n-2}{1} \right] + 1 \left[\binom{2}{2} + \binom{n-1}{2} \right],$$

$$\begin{aligned} \Sigma^1 n^2 &= 4 \left[-\binom{2}{1} + \binom{n-2}{1} \right] + 3 \left[\binom{2}{2} + \binom{n-1}{2} \right] \\ &\quad + 2 \left[-\binom{2}{3} + \binom{n}{3} \right]. \end{aligned}$$

$$\begin{aligned} \Sigma^1 n^3 &= 8 \left[-\binom{2}{1} + \binom{n-2}{1} \right] + 7 \left[\binom{2}{2} + \binom{n-1}{2} \right] \\ &\quad + 6 \left[-\binom{2}{3} + \binom{n}{3} \right] + 6 \left[\binom{2}{4} + \binom{n+1}{4} \right]. \end{aligned}$$

$$\begin{aligned} \Sigma^1 n^4 &= 16 \left[-\binom{2}{1} + \binom{n-2}{1} \right] + 15 \left[\binom{2}{2} + \binom{n-1}{2} \right] \\ &\quad + 14 \left[-\binom{2}{3} + \binom{n}{3} \right] + 12 \left[\binom{2}{4} + \binom{n+1}{4} \right] \\ &\quad + 24 \left[-\binom{2}{5} + \binom{n+2}{5} \right]. \end{aligned}$$

- For $t = 0$ the coefficients are $1, 0, 1, 0, -1, 2, 0, 1, -6, 6, \dots$ and registered in the OEIS [5] as [A278075](#).
- For $t = 1$ the coefficients are $1, 1, 1, 1, 1, 2, 1, 1, 0, 6, \dots$ and registered in the OEIS [5] as [A389570](#).
- For $t = 2$ the coefficients are $1, 2, 1, 4, 3, 2, 8, 7, 6, 6, \dots$ and registered in the OEIS [5] as [A391068](#).
- For $t = 3$ the coefficients are $1, 3, 1, 9, 5, 2, 27, 19, 12, 6, \dots$ and registered in the OEIS [5] as [A391210](#).

Lemma 1.4 (Backward differences in Eulerian numbers).

$$\Delta^j t^m = \sum_{k=0}^m \langle m \rangle_k \binom{t+k-j}{m-j}$$

Proof. By Worpitzky identity $t^m = \sum_{k=0}^m \langle m \rangle_k \binom{t+k}{m}$ and binomial recurrence $\binom{n+1}{k} = \binom{n}{k} + \binom{n}{k-1}$, see [6]. \square

Thus, let be a formula for ordinary sums of powers in terms of Eulerian numbers $\langle m \rangle_k$

Proposition 1.5 (Ordinary sums of powers in Eulerian numbers). *For non-negative integers n, m and an arbitrary integer t*

$$\Sigma^1 n^m = \sum_{j=0}^m \sum_{k=0}^m \left[(-1)^j \binom{t}{j+1} + \binom{j-t+n}{j+1} \right] \langle m \rangle_k \binom{t+k-j}{m-j}$$

Remarkable that having $t = 0$ formula for sums of powers turns into double binomial view

Proposition 1.6. *For non-negative integers n, m*

$$\Sigma^1 n^m = \sum_{j=0}^m \sum_{k=0}^m \binom{j+n}{j+1} \binom{k-j}{m-j} \langle m \rangle_k$$

Lemma 1.7 (Backward differences in Stirling numbers).

$$\nabla^j t^m = \sum_{k=j}^m \binom{t-j}{k-j} \left\{ m \right\}_k k!$$

Proof. By the identity $t^m = \sum_{k=0}^m \binom{t}{k} \{m\}_k k!$ and binomial recurrence $\binom{n+1}{k} = \binom{n}{k} + \binom{n}{k-1}$. \square

Thus, let be a formula for ordinary sums of powers in terms of Stirling numbers $\{m\}_k$

Proposition 1.8 (Ordinary sums of powers in Stirling numbers). *For non-negative integers n, m and an arbitrary integer t*

$$\Sigma^1 n^m = \sum_{j=0}^m \sum_{k=j}^m \left[(-1)^j \binom{t}{j+1} + \binom{j-t+n}{j+1} \right] \binom{t-j}{k-j} \{m\}_k k!$$

By setting $t = 0$ yields

Proposition 1.9. *For non-negative integers n, m*

$$\Sigma^1 n^m = \sum_{j=0}^m \sum_{k=j}^m \binom{j+n}{j+1} \binom{-j}{k-j} \{m\}_k k!$$

Formula for double sums of powers can be derived in a similar manner, by applying summation to the proposition (1.3), which in turn implies generalized hockey-stick identity, thus

$$\Sigma^2 n^m = \sum_{j=0}^m \nabla^j t^m \left[(-1)^j \binom{t}{j+1} \sum_{k=1}^n 1 + \sum_{k=1}^n \binom{j-t+k}{j+1} \right]$$

By applying generalized hockey stick identity (1.2), we obtain

$$\sum_{k=1}^n \binom{j-t+k}{j+1} = \sum_{k=j-t+1}^{j-t+n} \binom{k}{j+1} = \binom{j-t+n+1}{j+2} - \binom{j-t+1}{j+2}$$

Therefore,

$$\Sigma^2 n^m = \sum_{j=0}^m \nabla^j t^m \left[(-1)^j \binom{t}{j+1} n + \left(\binom{j-t+n+1}{j+2} - \binom{j-t+1}{j+2} \right) \right]$$

By applying the identity for negative binomial coefficients $\binom{-k}{j} = (-1)^j \binom{j+k-1}{j}$, we get

$$\binom{-(t-j-1)}{j+2} = (-1)^{j+2} \binom{t}{j+2}$$

Hence,

Proposition 1.10 (Double sums of powers via backward differences). *For non-negative integers n, m and an arbitrary integer t*

$$\Sigma^2 n^m = \sum_{j=0}^m \nabla^j t^m \left[(-1)^j \binom{t}{j+1} n + (-1)^{j+1} \binom{t}{j+2} n^0 + \binom{j-t+n+1}{j+2} \right]$$

In general,

Theorem 1.11 (Multifold sums of powers via backward difference). *For non-negative integers r, n, m and an arbitrary integer t*

$$\Sigma^r n^m = \sum_{j=0}^m \nabla^j t^m \left[\binom{j-t+n+r-1}{j+r} + \sum_{s=0}^{r-1} (-1)^{j+s} \binom{t}{j+s+1} \Sigma^{r-1-s} n^0 \right]$$

We may observe that

Proposition 1.12 (Multifold sum of zero powers). *For integers r and n*

$$\Sigma^r n^0 = \binom{r+n-1}{r}$$

Proof. By hockey stick identity $\sum_{k=0}^t \binom{j+k}{j} = \binom{j+t+1}{j+1}$. □

Thus $\Sigma^{r-1-s} n^0 = \binom{r-s+n-2}{r-s-1}$, which implies

Proposition 1.13 (Multifold sums of powers via backward difference binomial form).

For non-negative integers r, n, m and an arbitrary integer t

$$\Sigma^r n^m = \sum_{j=0}^m \nabla^j t^m \left[\binom{j-t+n+r-1}{j+r} + \sum_{s=0}^{r-1} (-1)^{j+s} \binom{t}{j+s+1} \binom{r-s+n-2}{r-s-1} \right]$$

2. CONCLUSIONS

In this manuscript, we derived formulas for sums of powers via Newton's interpolation formula based on backward finite differences of powers. In addition, we noticed that backward differences are closely related to Eulerian numbers, and Stirling numbers of the second kind. Thus, we express formulas for sums of powers in terms of Eulerian numbers, and Stirling

numbers of the second kind. All the results are validated using `Mathematica` programs, see dedicated section below.

REFERENCES

- [1] Petro Kolosov. Newton's interpolation formula and sums of powers, December 2025. <https://doi.org/10.5281/zenodo.18040979>.
- [2] Petro Kolosov. Sums of powers via central finite differences and newton's formula, December 2025. <https://doi.org/10.5281/zenodo.18096789>.
- [3] Knuth, Donald E. Johann Faulhaber and sums of powers. *Mathematics of Computation*, 61(203):277–294, 1993. <https://arxiv.org/abs/math/9207222>.
- [4] Steffensen, Johan Frederik. *Interpolation*. Williams & Wilkins, 1927. <https://www.amazon.com/-/de/Interpolation-Second-Dover-Books-Mathematics-ebook/dp/B00GHQVON8>.
- [5] Sloane, Neil J.A. and others. The on-line encyclopedia of integer sequences, 2003. <https://oeis.org/>.
- [6] J. Worpitzky. Studien über die bernoullischen und eulerschen zahlen. *Journal für die reine und angewandte Mathematik*, 94:203–232, 1883. <http://eudml.org/doc/148532>.
- [7] Petro Kolosov. Mathematica programs for backward finite differences and newton's formula. <https://github.com/kolosovpetro/SumsOfPowersViaBackwardFiniteDifferencesAndNewtonFormula/tree/main/mathematica>, 2026. GitHub repository, Mathematica source files.

MATHEMATICA PROGRAMS

Use the *Mathematica* package [7] to validate the results

Mathematica Function	Validates / Prints
<code>MultifoldSumOfPowersRecurrence[r, n, m]</code>	Computes $\sum^r n^m$
<code>ValidateOrdinarySumsOfPowersViaBackwardDifferences[20]</code>	Validates Proposition (1.3)
<code>ValidateBackwardDifferencesInEulerianNumbers[20]</code>	Validates Lemma (1.4)
<code>ValidateOrdinarySumsOfPowersInEulerianNumbers[10]</code>	Validates Proposition (1.5)
<code>ValidateBackwardDifferencesInStirlingNumbers[20]</code>	Validates Lemma (1.7)
<code>ValidateOrdinarySumsOfPowersInStirlingNumbers[20]</code>	Validates Proposition (1.8)
<code>ValidateDoubleSumsOfPowersViaBackwardDifferences[10]</code>	Validates Proposition (1.10)
<code>ValidateMultifoldSumsOfPowersViaBackwardDifference[5]</code>	Validates Theorem (1.11)
<code>ValidateMultifoldSumsOfPowersBackwardDiffBinomialForm[5]</code>	Validates Proposition (1.13)

Version: Local-0.1.0

License: This work is licensed under a [CC BY 4.0 License](#).

Sources: github.com/kolosovpetro/SumsOfPowersViaBackwardDifferences

ORCID: [0000-0002-6544-8880](#)

DOI: [10.5281/zenodo.18118011](https://doi.org/10.5281/zenodo.18118011)

Email: kolosovp94@gmail.com

Email address: kolosovp94@gmail.com

SOFTWARE DEVELOPER, DEVOPS ENGINEER

URL: <https://kolosovpetro.github.io>